su.nsk.iae.rpl/src/su/nsk/iae/rpl/invpatterngenerator/OuterExtraInvariantFormula.java
@@ -5,8 +5,13 @@ import java.util.List;
 import su.nsk.iae.rpl.rPL.UpdateStateVariable;
 
 public interface OuterExtraInvariantFormula extends OuterFormula {
-	public abstract LemmaPremise generateL8(UpdateStateVariable initState, UpdateStateVariable finalState);
-	public abstract LemmaPremise generateL9(OuterRequirementFormula reqFormula, UpdateStateVariable state);
+	LemmaPremise generateL8(UpdateStateVariable initState, UpdateStateVariable finalState);
+	LemmaPremise generateL9(OuterRequirementFormula reqFormula, UpdateStateVariable state);
+	String generateProofScriptForL8(
+			UpdateStateVariable initState, UpdateStateVariable finalState, ProofScriptGenerator generator);
+	String generateProofScriptForL9(
+			OuterRequirementFormula reqFormula, UpdateStateVariable state, ProofScriptGenerator generator);
+	
 	
 	public abstract String convertToString(UpdateStateVariable finalState);
 	
