su.nsk.iae.rpl/example_Patterns.thy
@@ -1,42 +1,50 @@
 theory example_Patterns imports Patterns
  begin
-definition always2 where "always2 A11 A12 A2 s \<equiv> (always (\<lambda> r2 r1 . ((weak_previous (\<lambda> r4 r3 . (\<not> (A11 r3))) r2 r1) \<or> ((\<not> (A12 r1)) \<or> (A2 r2 r1)))) s)"
+definition always2 where "always2 A11 A12 A2 s \<equiv> ((always (\<lambda> r2 r1 . ((weak_previous (\<lambda> r4 r3 . (\<not> (A11 r3))) r2 r1) \<or> ((\<not> (A12 r1)) \<or> (A2 r2 r1)))) s) \<and>(always (\<lambda> r2 r1 . ((weak_previous (\<lambda> r4 r3 . (\<not> (A11 r3))) r2 r1) \<or> ((\<not> (A12 r1)) \<or> (A2 r2 r1)))) s))"
 
 definition always2_part where "always2_part A11 A12 A2 s \<equiv> (always2 A11 A12 (\<lambda> s s1 . (A2 s1)) s)"
 
-definition always2_inv where "always2_inv b_0 A11 A12 A2_1 s \<equiv> ((always_inv (\<lambda> r2 r1 . ((weak_previous (\<lambda> r4 r3 . (\<not> (A11 r3))) r2 r1) \<or> ((\<not> (A12 r1)) \<or> (A2_1 r2 r1)))) s) \<and> (previous_inv b_0 (\<lambda> r4 r3 . (\<not> (A11 r3))) s))"
+definition always2_inv where "always2_inv b_0 b_1 A11 A12 A2_1 s \<equiv> (((always_inv (\<lambda> r2 r1 . ((weak_previous (\<lambda> r4 r3 . (\<not> (A11 r3))) r2 r1) \<or> ((\<not> (A12 r1)) \<or> (A2_1 r2 r1)))) s) \<and> (previous_inv b_0 (\<lambda> r4 r3 . (\<not> (A11 r3))) s)) \<and> ((always_inv (\<lambda> r2 r1 . ((weak_previous (\<lambda> r4 r3 . (\<not> (A11 r3))) r2 r1) \<or> ((\<not> (A12 r1)) \<or> (A2_1 r2 r1)))) s) \<and> (previous_inv b_1 (\<lambda> r4 r3 . (\<not> (A11 r3))) s)))"
 
-definition always2_inv_part where "always2_inv_part b_0 A11 A12 A2 s \<equiv> (always2_inv b_0 A11 A12 (\<lambda> s s1 . (A2 s1)) s)"
-
-
+definition always2_inv_part where "always2_inv_part b_0 b_1 A11 A12 A2 s \<equiv> (always2_inv b_0 b_1 A11 A12 (\<lambda> s s1 . (A2 s1)) s)"
 
 lemma always2_inv_saving_gen: "
-always2_inv b_0 A11 A12 A2_1 s0 \<Longrightarrow>
+always2_inv b_0 b_1 A11 A12 A2_1 s0 \<Longrightarrow>
 consecutive s0 s \<Longrightarrow>
-(((True \<and> (True \<and> (always_imp s0 (\<lambda> r1 . (A2_1 s0 r1)) (\<lambda> r1 . (A2_1 s r1))))) \<and> (((b_0 s0) \<and> True) \<or> ((\<not> (A12 s)) \<or> (A2_1 s s)))) \<and> ((b_0 s) --> (\<not> (A11 s)))) \<Longrightarrow>
-always2_inv b_0 A11 A12 A2_1 s"
+((((True \<and> (True \<and> (always_imp s0 (\<lambda> r1 . (A2_1 s0 r1)) (\<lambda> r1 . (A2_1 s r1))))) \<and> (((b_0 s0) \<and> True) \<or> ((\<not> (A12 s)) \<or> (A2_1 s s)))) \<and> ((b_0 s) --> (\<not> (A11 s)))) \<and> (((True \<and> (True \<and> (always_imp s0 (\<lambda> r1 . (A2_1 s0 r1)) (\<lambda> r1 . (A2_1 s r1))))) \<and> (((b_1 s0) \<and> True) \<or> ((\<not> (A12 s)) \<or> (A2_1 s s)))) \<and> ((b_1 s) --> (\<not> (A11 s))))) \<Longrightarrow>
+always2_inv b_0 b_1 A11 A12 A2_1 s"
+apply(erule conjE)
+apply(erule conjE)
+subgoal premises prems1
+apply(rule conjI)
+apply(insert prems1(1,2,4))[1]
+  sorry
+apply(insert prems1(1,3,5))
+  sorry
+done
+
 
 lemma always2einv_imp_req_gen: "
-always2_inv b_0 A11 A12 A2_1 s0 \<Longrightarrow>
+always2_inv b_0 b_1 A11 A12 A2_1 s0 \<Longrightarrow>
 toEnvP s0 \<Longrightarrow>
-(True \<and> (True \<and> (always_imp s0 (\<lambda> r1 . (A2_1 s0 r1)) (\<lambda> r1 . (A2 s0 r1))))) \<Longrightarrow>
+((True \<and> (True \<and> (always_imp s0 (\<lambda> r1 . (A2_1 s0 r1)) (\<lambda> r1 . (A2 s0 r1))))) \<and> (True \<and> (True \<and> (always_imp s0 (\<lambda> r1 . (A2_1 s0 r1)) (\<lambda> r1 . (A2 s0 r1)))))) \<Longrightarrow>
 always2 A11 A12 A2 s0"
 
 lemma always2_inv_saving: "
-always2_inv_part b_0 A11 A12 A2 s0 \<Longrightarrow>
+always2_inv_part b_0 b_1 A11 A12 A2 s0 \<Longrightarrow>
 consecutive s0 s \<Longrightarrow>
-(((b_0 s0) \<or> ((\<not> (A12 s)) \<or> (A2 s))) \<and> ((b_0 s) --> (\<not> (A11 s)))) \<Longrightarrow>
-always2_inv_part b_0 A11 A12 A2 s"
+((((b_0 s0) \<or> ((\<not> (A12 s)) \<or> (A2 s))) \<and> ((b_0 s) --> (\<not> (A11 s)))) \<and> (((b_1 s0) \<or> ((\<not> (A12 s)) \<or> (A2 s))) \<and> ((b_1 s) --> (\<not> (A11 s))))) \<Longrightarrow>
+always2_inv_part b_0 b_1 A11 A12 A2 s"
 
 lemma always2einv_imp_req: "
-always2_inv_part b_0 A11 A12 A2 s \<Longrightarrow>
+always2_inv_part b_0 b_1 A11 A12 A2 s \<Longrightarrow>
 toEnvP s \<Longrightarrow>
 True \<Longrightarrow>
 always2_part A11 A12 A2 s"
 
-lemmas always2_used_patterns = always2_def always_def weak_previous_def 
+lemmas always2_used_patterns = always2_def always_def weak_previous_def always_def weak_previous_def 
 
-lemmas always2_inv_used_patterns = always2_inv_def always_inv_def weak_previous_def previous_inv_def 
+lemmas always2_inv_used_patterns = always2_inv_def always_inv_def weak_previous_def previous_inv_def always_inv_def weak_previous_def previous_inv_def 
 
 lemmas always2_inv_part_used_patterns = always2_inv_part_def always2_inv_used_patterns
 
@@ -50,13 +58,12 @@ definition P1_1_inv where "P1_1_inv t t1_0 A1 A2_1 A3_1 s \<equiv> (always_inv (
 
 definition P1_1_inv_part where "P1_1_inv_part t t1_0 A1 A2 A3 s \<equiv> (P1_1_inv t t1_0 A1 (\<lambda> s s1 . (A2 s1)) (\<lambda> s s1 . (A3 s1)) s)"
 
-
-
 lemma P1_1_inv_saving_gen: "
 P1_1_inv t t1_0 A1 A2_1 A3_1 s0 \<Longrightarrow>
 consecutive s0 s \<Longrightarrow>
 ((True \<and> ((always_imp s0 (A2_1 s0) (A2_1 s)) \<and> ((always_imp s0 (A3_1 s0) (A3_1 s)) \<and> (((t1_0 s0) = 0) \<or> (((A3_1 s s) \<and> ((t1_0 s0) <= t)) \<or> ((A2_1 s s) \<and> ((t1_0 s0) < (t1_0 s)))))))) \<and> ((\<not> (A1 s)) \<or> ((A3_1 s s) \<or> ((A2_1 s s) \<and> ((t1_0 s) > 0))))) \<Longrightarrow>
 P1_1_inv t t1_0 A1 A2_1 A3_1 s"
+sorry
 
 lemma P1_1einv_imp_req_gen: "
 P1_1_inv t t1_0 A1 A2_1 A3_1 s0 \<Longrightarrow>
@@ -92,13 +99,12 @@ definition P1_2_inv where "P1_2_inv t b_0 t1_0 A11 A12 A2_1 A3_1 s \<equiv> ((al
 
 definition P1_2_inv_part where "P1_2_inv_part t b_0 t1_0 A11 A12 A2 A3 s \<equiv> (P1_2_inv t b_0 t1_0 A11 A12 (\<lambda> s s1 . (A2 s1)) (\<lambda> s s1 . (A3 s1)) s)"
 
-
-
 lemma P1_2_inv_saving_gen: "
 P1_2_inv t b_0 t1_0 A11 A12 A2_1 A3_1 s0 \<Longrightarrow>
 consecutive s0 s \<Longrightarrow>
 (((True \<and> (True \<and> ((always_imp s0 (A2_1 s0) (A2_1 s)) \<and> ((always_imp s0 (A3_1 s0) (A3_1 s)) \<and> (((t1_0 s0) = 0) \<or> (((A3_1 s s) \<and> ((t1_0 s0) <= t)) \<or> ((A2_1 s s) \<and> ((t1_0 s0) < (t1_0 s))))))))) \<and> (((b_0 s0) \<and> True) \<or> ((\<not> (A12 s)) \<or> ((A3_1 s s) \<or> ((A2_1 s s) \<and> ((t1_0 s) > 0)))))) \<and> ((b_0 s) --> (\<not> (A11 s)))) \<Longrightarrow>
 P1_2_inv t b_0 t1_0 A11 A12 A2_1 A3_1 s"
+sorry
 
 lemma P1_2einv_imp_req_gen: "
 P1_2_inv t b_0 t1_0 A11 A12 A2_1 A3_1 s0 \<Longrightarrow>
@@ -134,13 +140,12 @@ definition P2_1_inv where "P2_1_inv t t1_0 A1 A2_1 s \<equiv> (always_inv (\<lam
 
 definition P2_1_inv_part where "P2_1_inv_part t t1_0 A1 A2 s \<equiv> (P2_1_inv t t1_0 A1 (\<lambda> s s1 . (A2 s1)) s)"
 
-
-
 lemma P2_1_inv_saving_gen: "
 P2_1_inv t t1_0 A1 A2_1 s0 \<Longrightarrow>
 consecutive s0 s \<Longrightarrow>
 ((True \<and> ((t = 0) \<or> ((always_imp s0 (A2_1 s0) (A2_1 s)) \<and> (((((t1_0 s0) + 1) >= t) \<or> (A2_1 s s)) \<and> ((t1_0 s) <= ((t1_0 s0) + 1)))))) \<and> ((\<not> (A1 s)) \<or> ((t = 0) \<or> (((t1_0 s) = 0) \<and> (A2_1 s s))))) \<Longrightarrow>
 P2_1_inv t t1_0 A1 A2_1 s"
+sorry
 
 lemma P2_1einv_imp_req_gen: "
 P2_1_inv t t1_0 A1 A2_1 s0 \<Longrightarrow>
@@ -176,13 +181,12 @@ definition P2_2_inv where "P2_2_inv t b_0 t1_0 A11 A12 A2_1 s \<equiv> ((always_
 
 definition P2_2_inv_part where "P2_2_inv_part t b_0 t1_0 A11 A12 A2 s \<equiv> (P2_2_inv t b_0 t1_0 A11 A12 (\<lambda> s s1 . (A2 s1)) s)"
 
-
-
 lemma P2_2_inv_saving_gen: "
 P2_2_inv t b_0 t1_0 A11 A12 A2_1 s0 \<Longrightarrow>
 consecutive s0 s \<Longrightarrow>
 (((True \<and> (True \<and> ((t = 0) \<or> ((always_imp s0 (A2_1 s0) (A2_1 s)) \<and> (((((t1_0 s0) + 1) >= t) \<or> (A2_1 s s)) \<and> ((t1_0 s) <= ((t1_0 s0) + 1))))))) \<and> (((b_0 s0) \<and> True) \<or> ((\<not> (A12 s)) \<or> ((t = 0) \<or> (((t1_0 s) = 0) \<and> (A2_1 s s)))))) \<and> ((b_0 s) --> (\<not> (A11 s)))) \<Longrightarrow>
 P2_2_inv t b_0 t1_0 A11 A12 A2_1 s"
+sorry
 
 lemma P2_2einv_imp_req_gen: "
 P2_2_inv t b_0 t1_0 A11 A12 A2_1 s0 \<Longrightarrow>
@@ -218,13 +222,12 @@ definition P3_1_inv where "P3_1_inv w_0 A1 A2_1 A3_1 s \<equiv> (always_inv (\<l
 
 definition P3_1_inv_part where "P3_1_inv_part w_0 A1 A2 A3 s \<equiv> (P3_1_inv w_0 A1 (\<lambda> s s1 . (A2 s1)) (\<lambda> s s1 . (A3 s1)) s)"
 
-
-
 lemma P3_1_inv_saving_gen: "
 P3_1_inv w_0 A1 A2_1 A3_1 s0 \<Longrightarrow>
 consecutive s0 s \<Longrightarrow>
 ((True \<and> ((always_imp s0 (A2_1 s0) (A2_1 s)) \<and> ((always_imp s0 (A3_1 s0) (A3_1 s)) \<and> ((\<not> (w_0 s0)) \<or> ((A3_1 s s) \<or> ((w_0 s) \<and> (A2_1 s s))))))) \<and> ((\<not> (A1 s)) \<or> ((A3_1 s s) \<or> ((w_0 s) \<and> (A2_1 s s))))) \<Longrightarrow>
 P3_1_inv w_0 A1 A2_1 A3_1 s"
+sorry
 
 lemma P3_1einv_imp_req_gen: "
 P3_1_inv w_0 A1 A2_1 A3_1 s0 \<Longrightarrow>
@@ -260,13 +263,12 @@ definition P3_2_inv where "P3_2_inv b_0 w_0 A11 A12 A2_1 A3_1 s \<equiv> ((alway
 
 definition P3_2_inv_part where "P3_2_inv_part b_0 w_0 A11 A12 A2 A3 s \<equiv> (P3_2_inv b_0 w_0 A11 A12 (\<lambda> s s1 . (A2 s1)) (\<lambda> s s1 . (A3 s1)) s)"
 
-
-
 lemma P3_2_inv_saving_gen: "
 P3_2_inv b_0 w_0 A11 A12 A2_1 A3_1 s0 \<Longrightarrow>
 consecutive s0 s \<Longrightarrow>
 (((True \<and> (True \<and> ((always_imp s0 (A2_1 s0) (A2_1 s)) \<and> ((always_imp s0 (A3_1 s0) (A3_1 s)) \<and> ((\<not> (w_0 s0)) \<or> ((A3_1 s s) \<or> ((w_0 s) \<and> (A2_1 s s)))))))) \<and> (((b_0 s0) \<and> True) \<or> ((\<not> (A12 s)) \<or> ((A3_1 s s) \<or> ((w_0 s) \<and> (A2_1 s s)))))) \<and> ((b_0 s) --> (\<not> (A11 s)))) \<Longrightarrow>
 P3_2_inv b_0 w_0 A11 A12 A2_1 A3_1 s"
+sorry
 
 lemma P3_2einv_imp_req_gen: "
 P3_2_inv b_0 w_0 A11 A12 A2_1 A3_1 s0 \<Longrightarrow>
@@ -302,13 +304,12 @@ definition P3_3_inv where "P3_3_inv b_0 w_0 A1 A2_1 A3_1 s \<equiv> ((always_inv
 
 definition P3_3_inv_part where "P3_3_inv_part b_0 w_0 A1 A2 A3 s \<equiv> (P3_3_inv b_0 w_0 A1 (\<lambda> s s1 . (A2 s1)) (\<lambda> s s1 . (A3 s1)) s)"
 
-
-
 lemma P3_3_inv_saving_gen: "
 P3_3_inv b_0 w_0 A1 A2_1 A3_1 s0 \<Longrightarrow>
 consecutive s0 s \<Longrightarrow>
 (((True \<and> ((always_imp s0 (A2_1 s0) (A2_1 s)) \<and> ((always_imp s0 (A3_1 s0) (A3_1 s)) \<and> ((\<not> (w_0 s0)) \<or> ((A3_1 s s) \<or> ((w_0 s) \<and> (A2_1 s s))))))) \<and> (((b_0 s0) \<and> True) \<or> ((A3_1 s s) \<or> ((w_0 s) \<and> (A2_1 s s))))) \<and> ((b_0 s) --> (\<not> (A1 s)))) \<Longrightarrow>
 P3_3_inv b_0 w_0 A1 A2_1 A3_1 s"
+sorry
 
 lemma P3_3einv_imp_req_gen: "
 P3_3_inv b_0 w_0 A1 A2_1 A3_1 s0 \<Longrightarrow>
@@ -344,13 +345,12 @@ definition P3_4_inv where "P3_4_inv b_0 b_1 w_0 A11 A12 A2_1 A3_1 s \<equiv> (((
 
 definition P3_4_inv_part where "P3_4_inv_part b_0 b_1 w_0 A11 A12 A2 A3 s \<equiv> (P3_4_inv b_0 b_1 w_0 A11 A12 (\<lambda> s s1 . (A2 s1)) (\<lambda> s s1 . (A3 s1)) s)"
 
-
-
 lemma P3_4_inv_saving_gen: "
 P3_4_inv b_0 b_1 w_0 A11 A12 A2_1 A3_1 s0 \<Longrightarrow>
 consecutive s0 s \<Longrightarrow>
 (((((True \<and> True) \<and> ((always_imp s0 (A2_1 s0) (A2_1 s)) \<and> ((always_imp s0 (A3_1 s0) (A3_1 s)) \<and> ((\<not> (w_0 s0)) \<or> ((A3_1 s s) \<or> ((w_0 s) \<and> (A2_1 s s))))))) \<and> (((b_1 s0) \<and> (True \<and> True)) \<or> ((A3_1 s s) \<or> ((w_0 s) \<and> (A2_1 s s))))) \<and> ((b_1 s) --> (((b_0 s0) \<and> True) \<or> (\<not> (A12 s))))) \<and> ((b_0 s) --> (\<not> (A11 s)))) \<Longrightarrow>
 P3_4_inv b_0 b_1 w_0 A11 A12 A2_1 A3_1 s"
+sorry
 
 lemma P3_4einv_imp_req_gen: "
 P3_4_inv b_0 b_1 w_0 A11 A12 A2_1 A3_1 s0 \<Longrightarrow>
@@ -386,13 +386,12 @@ definition P4_1_inv where "P4_1_inv t t1_0 A1 A2_1 A3_1 s \<equiv> (always_inv (
 
 definition P4_1_inv_part where "P4_1_inv_part t t1_0 A1 A2 A3 s \<equiv> (P4_1_inv t t1_0 A1 (\<lambda> s s1 . (A2 s1)) (\<lambda> s s1 . (A3 s1)) s)"
 
-
-
 lemma P4_1_inv_saving_gen: "
 P4_1_inv t t1_0 A1 A2_1 A3_1 s0 \<Longrightarrow>
 consecutive s0 s \<Longrightarrow>
 ((True \<and> ((always_imp s0 (A2_1 s0) (A2_1 s)) \<and> ((always_imp s0 (A3_1 s0) (A3_1 s)) \<and> ((((t1_0 s0) < t) \<and> (((A3_1 s s) \<and> ((t1_0 s) <= (t + 1))) \<or> (((t1_0 s) <= ((t1_0 s0) + 1)) \<and> (A2_1 s s)))) \<or> (((t1_0 s0) >= t) \<and> ((t1_0 s) <= ((t1_0 s0) + 1))))))) \<and> ((\<not> (A1 s)) \<or> ((A3_1 s s) \<or> (((t1_0 s) = 0) \<and> (A2_1 s s))))) \<Longrightarrow>
 P4_1_inv t t1_0 A1 A2_1 A3_1 s"
+sorry
 
 lemma P4_1einv_imp_req_gen: "
 P4_1_inv t t1_0 A1 A2_1 A3_1 s0 \<Longrightarrow>
@@ -428,13 +427,12 @@ definition P4_2_inv where "P4_2_inv t b_0 t1_0 A11 A12 A2_1 A3_1 s \<equiv> ((al
 
 definition P4_2_inv_part where "P4_2_inv_part t b_0 t1_0 A11 A12 A2 A3 s \<equiv> (P4_2_inv t b_0 t1_0 A11 A12 (\<lambda> s s1 . (A2 s1)) (\<lambda> s s1 . (A3 s1)) s)"
 
-
-
 lemma P4_2_inv_saving_gen: "
 P4_2_inv t b_0 t1_0 A11 A12 A2_1 A3_1 s0 \<Longrightarrow>
 consecutive s0 s \<Longrightarrow>
 (((True \<and> (True \<and> ((always_imp s0 (A2_1 s0) (A2_1 s)) \<and> ((always_imp s0 (A3_1 s0) (A3_1 s)) \<and> ((((t1_0 s0) < t) \<and> (((A3_1 s s) \<and> ((t1_0 s) <= (t + 1))) \<or> (((t1_0 s) <= ((t1_0 s0) + 1)) \<and> (A2_1 s s)))) \<or> (((t1_0 s0) >= t) \<and> ((t1_0 s) <= ((t1_0 s0) + 1)))))))) \<and> (((b_0 s0) \<and> True) \<or> ((\<not> (A12 s)) \<or> ((A3_1 s s) \<or> (((t1_0 s) = 0) \<and> (A2_1 s s)))))) \<and> ((b_0 s) --> (\<not> (A11 s)))) \<Longrightarrow>
 P4_2_inv t b_0 t1_0 A11 A12 A2_1 A3_1 s"
+sorry
 
 lemma P4_2einv_imp_req_gen: "
 P4_2_inv t b_0 t1_0 A11 A12 A2_1 A3_1 s0 \<Longrightarrow>
@@ -470,13 +468,12 @@ definition P4_3_inv where "P4_3_inv t b_0 b_1 t1_0 A11 A12 A21_1 A22_1 A3_1 s \<
 
 definition P4_3_inv_part where "P4_3_inv_part t b_0 b_1 t1_0 A11 A12 A21 A22 A3 s \<equiv> (P4_3_inv t b_0 b_1 t1_0 A11 A12 (\<lambda> s s1 . (A21 s1)) (\<lambda> s s1 . (A22 s1)) (\<lambda> s s1 . (A3 s1)) s)"
 
-
-
 lemma P4_3_inv_saving_gen: "
 P4_3_inv t b_0 b_1 t1_0 A11 A12 A21_1 A22_1 A3_1 s0 \<Longrightarrow>
 consecutive s0 s \<Longrightarrow>
 ((((True \<and> (True \<and> (((always_imp s0 (A21_1 s0) (A21_1 s)) \<and> (always_imp s0 (\<lambda> r3 . (A22_1 s0 r3)) (\<lambda> r3 . (A22_1 s r3)))) \<and> ((always_imp s0 (A3_1 s0) (A3_1 s)) \<and> ((((t1_0 s0) < t) \<and> (((A3_1 s s) \<and> ((t1_0 s) <= (t + 1))) \<or> (((t1_0 s) <= ((t1_0 s0) + 1)) \<and> (((b_1 s0) \<and> (always_imp s0 (A21_1 s0) (A21_1 s))) \<and> (A22_1 s s))))) \<or> (((t1_0 s0) >= t) \<and> ((t1_0 s) <= ((t1_0 s0) + 1)))))))) \<and> (((b_0 s0) \<and> True) \<or> ((\<not> (A12 s)) \<or> ((A3_1 s s) \<or> (((t1_0 s) = 0) \<and> (((b_1 s0) \<and> (always_imp s0 (A21_1 s0) (A21_1 s))) \<and> (A22_1 s s))))))) \<and> ((b_0 s) --> (\<not> (A11 s)))) \<and> ((b_1 s) --> (A21_1 s s))) \<Longrightarrow>
 P4_3_inv t b_0 b_1 t1_0 A11 A12 A21_1 A22_1 A3_1 s"
+sorry
 
 lemma P4_3einv_imp_req_gen: "
 P4_3_inv t b_0 b_1 t1_0 A11 A12 A21_1 A22_1 A3_1 s0 \<Longrightarrow>
@@ -512,13 +509,12 @@ definition P6_1_inv where "P6_1_inv t b_0 t1_0 b_1 A1 A2 A3 A4_1 s \<equiv> (((a
 
 definition P6_1_inv_part where "P6_1_inv_part t b_0 t1_0 b_1 A1 A2 A3 A4 s \<equiv> (P6_1_inv t b_0 t1_0 b_1 A1 A2 A3 (\<lambda> s s1 . (A4 s1)) s)"
 
-
-
 lemma P6_1_inv_saving_gen: "
 P6_1_inv t b_0 t1_0 b_1 A1 A2 A3 A4_1 s0 \<Longrightarrow>
 consecutive s0 s \<Longrightarrow>
 (((((True \<and> True) \<and> (True \<and> (always_imp s0 (\<lambda> r1 . (A4_1 s0 r1)) (\<lambda> r1 . (A4_1 s r1))))) \<and> (((b_1 s0) \<and> (True \<and> True)) \<or> ((\<not> (A3 s)) \<or> (A4_1 s s)))) \<and> ((b_1 s) --> (((t > 0) \<or> (\<not> (A1 s))) \<and> ((\<not> (A2 s)) \<or> ((b_0 s0) \<and> (True \<and> (True \<and> ((t1_0 s0) < t)))))))) \<and> ((((t1_0 s) > 0) \<or> (\<not> (A1 s))) \<and> ((\<not> (A2 s)) \<or> ((b_0 s0) \<and> (True \<and> (True \<and> ((t1_0 s0) < (t1_0 s)))))))) \<Longrightarrow>
 P6_1_inv t b_0 t1_0 b_1 A1 A2 A3 A4_1 s"
+sorry
 
 lemma P6_1einv_imp_req_gen: "
 P6_1_inv t b_0 t1_0 b_1 A1 A2 A3 A4_1 s0 \<Longrightarrow>
@@ -554,13 +550,12 @@ definition P6_2_inv where "P6_2_inv t b_0 t1_0 b_1 w_0 A1 A2 A3 A4_1 A5_1 s \<eq
 
 definition P6_2_inv_part where "P6_2_inv_part t b_0 t1_0 b_1 w_0 A1 A2 A3 A4 A5 s \<equiv> (P6_2_inv t b_0 t1_0 b_1 w_0 A1 A2 A3 (\<lambda> s s1 . (A4 s1)) (\<lambda> s s1 . (A5 s1)) s)"
 
-
-
 lemma P6_2_inv_saving_gen: "
 P6_2_inv t b_0 t1_0 b_1 w_0 A1 A2 A3 A4_1 A5_1 s0 \<Longrightarrow>
 consecutive s0 s \<Longrightarrow>
 (((((True \<and> True) \<and> (True \<and> ((always_imp s0 (A4_1 s0) (A4_1 s)) \<and> ((always_imp s0 (A5_1 s0) (A5_1 s)) \<and> ((\<not> (w_0 s0)) \<or> ((A5_1 s s) \<or> ((w_0 s) \<and> (A4_1 s s)))))))) \<and> (((b_1 s0) \<and> (True \<and> True)) \<or> ((\<not> (A3 s)) \<or> ((A5_1 s s) \<or> ((w_0 s) \<and> (A4_1 s s)))))) \<and> ((b_1 s) --> (((t > 0) \<or> (\<not> (A1 s))) \<and> ((\<not> (A2 s)) \<or> ((b_0 s0) \<and> (True \<and> (True \<and> ((t1_0 s0) < t)))))))) \<and> ((((t1_0 s) > 0) \<or> (\<not> (A1 s))) \<and> ((\<not> (A2 s)) \<or> ((b_0 s0) \<and> (True \<and> (True \<and> ((t1_0 s0) < (t1_0 s)))))))) \<Longrightarrow>
 P6_2_inv t b_0 t1_0 b_1 w_0 A1 A2 A3 A4_1 A5_1 s"
+sorry
 
 lemma P6_2einv_imp_req_gen: "
 P6_2_inv t b_0 t1_0 b_1 w_0 A1 A2 A3 A4_1 A5_1 s0 \<Longrightarrow>
