su.nsk.iae.rpl/src/su/nsk/iae/rpl/invpatterngenerator/ProofScriptGenerator.xtend
@@ -1,0 +1,190 @@
+package su.nsk.iae.rpl.invpatterngenerator
+
+import su.nsk.iae.rpl.rPL.UpdateStateVariable
+import java.util.ListIterator
+import java.util.ArrayList
+import su.nsk.iae.rpl.rPL.PastExtraInvariantPattern
+
+class ProofScriptGenerator {
+	int premisesNumber;
+	static final String BASE_PREMISES_NAME = "prems";
+	
+	def String generateForOuterConjunction(
+		OuterExtraInvariantFormula left, OuterExtraInvariantFormula right, UpdateStateVariable initState, UpdateStateVariable finalState
+	) {
+		premisesNumber++;
+		val premisesName = BASE_PREMISES_NAME + premisesNumber;
+		return '''
+		apply(erule conjE)
+		apply(erule conjE)
+		subgoal premises «premisesName»
+		apply(rule conjI)
+		apply(insert «premisesName»(1,2,4))[1]
+		  «left.generateProofScriptForL8(initState, finalState, this)»
+		apply(insert «premisesName»(1,3,5))
+		  «right.generateProofScriptForL8(initState, finalState, this)»
+		done
+		'''
+	}
+	
+	def String generateForOuterDisjunction(
+		OuterExtraInvariantFormula left, OuterExtraInvariantFormula right, UpdateStateVariable initState, UpdateStateVariable finalState
+	) {
+		premisesNumber++;
+		val premisesName = BASE_PREMISES_NAME + premisesNumber;
+		return '''
+		apply(erule conjE)
+		subgoal premises «premisesName»
+		apply(insert «premisesName»(1,2)
+		apply(erule disjE)
+		apply(insert «premisesName»(3)
+		apply(rule disjI1)
+		  «left.generateProofScriptForL8(initState, finalState, this)»
+		apply(insert «premisesName»(4)
+		apply(rule disjI2)
+		  «right.generateProofScriptForL8(initState, finalState, this)»
+		done
+		'''
+	}
+	
+	def String generateForOuterConjunction(
+		OuterExtraInvariantFormula left, OuterExtraInvariantFormula right, OuterRequirementFormula reqLeft,
+		OuterRequirementFormula reqRight, UpdateStateVariable state
+	) {
+		premisesNumber++;
+		val premisesName = BASE_PREMISES_NAME + premisesNumber;
+		return '''
+		apply(erule conjE)
+		apply(erule conjE)
+		subgoal premises «premisesName»
+		apply(rule conjI)
+		apply(insert «premisesName»(1,2,4))[1]
+		  «left.generateProofScriptForL9(reqLeft, state, this)»
+		apply(insert «premisesName»(1,3,5))
+		  «right.generateProofScriptForL9(reqRight, state, this)»
+		done
+		'''
+	}
+	
+	def String generateForOuterDisjunction(
+		OuterExtraInvariantFormula left, OuterExtraInvariantFormula right, OuterRequirementFormula reqLeft,
+		OuterRequirementFormula reqRight, UpdateStateVariable state
+	) {
+		premisesNumber++;
+		val premisesName = BASE_PREMISES_NAME + premisesNumber;
+		return '''
+		apply(erule conjE)
+		subgoal premises «premisesName»
+		apply(insert «premisesName»(1,2)
+		apply(erule disjE)
+		apply(insert «premisesName»(3)
+		apply(rule disjI1)
+		  «left.generateProofScriptForL9(reqLeft, state, this)»
+		apply(insert «premisesName»(4)
+		apply(rule disjI2)
+		  «right.generateProofScriptForL9(reqRight, state, this)»
+		done
+		'''
+	}
+	
+	def String generateForExtendedInvariant(
+		ExtendedInvariant extraInv, UpdateStateVariable initState, UpdateStateVariable finalState
+	) {
+		val extraConjs = extraInv.getExtraConjs();
+		val iter = extraConjs.listIterator(extraConjs.size());
+		val script = new StringBuilder();
+		val premisesNames = new ArrayList();
+		while (iter.hasPrevious()) {
+			premisesNumber++;
+			val premisesName = BASE_PREMISES_NAME + premisesNumber;
+			val extraConj = iter.previous();
+			extraConj.setName(premisesName + "(3)");
+			premisesNames.add(premisesName);
+			script.append('''
+			apply(erule conjE)
+			apply(erule conjE)
+			subgoal premises «premisesName»
+			apply(insert «premisesName»(1,2,4)[1]
+			''');
+		}
+		script.append('''
+		apply(erule «extraInv.getMainConj().getPattern().getLemmas().getL8().getName()»)
+		  apply simp
+		  «extraInv.generateL8PremiseInstance(initState, finalState).generateProofScript(this)»
+		''');
+		for (PastExtraInvariantPatternInstance extraConj: extraConjs) {
+			val premisesName = premisesNames.remove(premisesNames.size() -1);
+			script.append('''
+			apply(insert «premisesName»(1,3,5)
+			  apply(erule «extraConj.getPattern().getLemmas().getL6().getName()»
+			  apply simp
+			  «extraConj.generateLemmaPremiseInstance(initState).generateProofScript(this)»
+			done
+			''')
+		}
+		return script.toString();
+	}
+	
+	def String generateForDerivedRequirementPatternInstance(
+		ExtendedInvariant extraInvFormula, DerivedRequirementPatternInstance reqFormula, UpdateStateVariable state
+	) {
+		val extraConjs = extraInvFormula.getExtraConjs();
+		premisesNumber++;
+		val premises1 = BASE_PREMISES_NAME + premisesNumber;
+		premisesNumber++;
+		val premises2 = BASE_PREMISES_NAME + premisesNumber;
+		return '''
+		«IF extraConjs.size() > 0»
+		subgoal premises «premises1»
+		apply(insert «premises1»(1,2))
+		«IF extraConjs.size() > 1»
+		apply(simp only: conj_assoc)
+		«ENDIF»
+		apply(erule conjE)
+		subgoal premises «premises2»
+		apply(insert «premises2»(1,2) «premises1»(3))
+		«ENDIF»
+		apply(erule «reqFormula.getL9().getName()»
+		apply simp
+		  «extraInvFormula.generateL9PremiseInstance(reqFormula, state).generateProofScript(this)»
+		«IF extraConjs.size() > 0»
+		done
+		done
+		«ENDIF»
+		'''		
+	}
+	
+	def String generateForLemmaPremiseConjunction(LemmaPremise left, LemmaPremise right) {
+		premisesNumber++;
+		val premisesName = BASE_PREMISES_NAME + premisesNumber;
+		return '''
+		apply(erule conjE)
+		apply(erule conjE)
+		subgoal premises «premisesName»
+		apply(rule conjI)
+		apply(insert «premisesName»(1,2)[1]
+		  «left.generateProofScript(this)»
+		apply(insert «premisesName»(1,3)
+		  «right.generateProofScript(this)»
+		done
+		'''
+	}
+	
+	def String generateForLemmaPremiseDisjunction(LemmaPremise left, LemmaPremise right) {
+		return '''
+		apply(erule disjE)
+		apply(rule disjI1)
+		  «left.generateProofScript(this)»
+		apply(rule disjI2)
+		  «right.generateProofScript(this)»
+		'''
+	}
+	
+	def generateForFutureExtraInvariantPatternInstance(FutureExtraInvariantPatternInstance patternInst) {
+		return '''
+		apply(rule «patternInst.getPattern().getLemmas().getL2().getName()»)
+		apply simp
+		  «patternInst.generateLemmaPremiseInstance().generateProofScript(this)»
+		'''
+	}
+}
